hash_160

Opcodes.fst
@@ -10,9 +10,10 @@ module List = FStar.List.Tot
 (* 76 A9 14 ... 88 AC *)
 
 
+assume val hash_sha256: #a: eqtype -> input : a -> Tot(output : a)
+assume val hash_ripemd160: #a:eqtype -> input : a -> Tot(output: a)
+
 (* 118 *)
-
-
 val op_dup : #a: eqtype -> st_before: stackBC a{Stack.length st_before > 0 /\ Stack.capacity st_before > 0}  -> 
 				line_before: seq nat{Seq.length line_before > 0 /\ (Seq.head line_before = 118)}
 				-> Tot (st: stackBC a 
@@ -29,3 +30,18 @@ let op_dup #a st_before line_before =
 	let stack_push2 = Stack.push stack_push1 element in 
 	let line = Seq.tail line_before in (stack_push2, line)
 
+val op_hash160 : #a: eqtype -> st_before : stackBC a{Stack.length st_before > 0} -> 
+				line_before : seq nat {Seq.length line_before > 0 /\ (Seq.head line_before = 169)}
+				-> Tot(st: stackBC a 
+						{Stack.length st > 0  /\
+						Stack.index st 0 = (hash_ripemd160(hash_sha256 (Stack.index st_before 0))) /\
+						Stack.length st = Stack.length st_before} * 
+					line : seq nat {Seq.length line = Seq.length line_before - 1})
+
+let op_hash160 #a st_before line_before = 
+	let pop = Stack.pop st_before in 
+	let element = fst pop in 
+	let stack_after_pop = snd pop in 
+	let element = hash_ripemd160(hash_sha256 element) in 
+	let stack_push1 = Stack.push stack_after_pop element in 
+	let line = Seq.tail line_before in (stack_push1, line)
